Renaming planes and positions

opentheory/theories/char/char.ml
@@ -19,69 +19,71 @@ logfile "char-def";;
 (* Planes *)
 (* ~~~~~~ *)
 
-let is_plane_def = new_definition
-  `!p. is_plane p = byte_lt p (num_to_byte 17)`;;
+let is_unicode_plane_def = new_definition
+  `!p. is_unicode_plane p = byte_lt p (num_to_byte 17)`;;
 
-export_thm is_plane_def;;
+export_thm is_unicode_plane_def;;
 
-let plane_exists = prove
-  (`?p. is_plane p`,
+let unicode_plane_exists = prove
+  (`?p. is_unicode_plane p`,
    EXISTS_TAC `num_to_byte 0` THEN
-   REWRITE_TAC [is_plane_def] THEN
+   REWRITE_TAC [is_unicode_plane_def] THEN
    CONV_TAC byte_reduce_conv);;
 
-let (plane_abs_rep,plane_rep_abs) =
+let (unicode_plane_abs_rep,unicode_plane_rep_abs) =
   let tybij =
-    new_type_definition "plane" ("mk_plane","dest_plane") plane_exists in
+    new_type_definition "unicode_plane"
+      ("mk_unicode_plane","dest_unicode_plane") unicode_plane_exists in
   CONJ_PAIR tybij;;
 
-export_thm plane_abs_rep;;
-export_thm plane_rep_abs;;
+export_thm unicode_plane_abs_rep;;
+export_thm unicode_plane_rep_abs;;
 
-let plane_tybij = CONJ plane_abs_rep plane_rep_abs;;
+let unicode_plane_tybij = CONJ unicode_plane_abs_rep unicode_plane_rep_abs;;
 
-let rdecode_plane_def = new_definition
+let rdecode_unicode_plane_def = new_definition
   `!r.
-     rdecode_plane r =
+     rdecode_unicode_plane r =
      let (n,r') = rdecode_uniform 17 r in
-     (mk_plane (num_to_byte n), r')`;;
+     (mk_unicode_plane (num_to_byte n), r')`;;
 
-export_thm rdecode_plane_def;;
+export_thm rdecode_unicode_plane_def;;
 
 (* ~~~~~~~~~ *)
 (* Positions *)
 (* ~~~~~~~~~ *)
 
-let is_position_def =
+let is_unicode_position_def =
   let def = new_definition
-    `!p. is_position (p : word16) = T` in
+    `!p. is_unicode_position (p : word16) = T` in
   REWRITE_RULE [] def;;
 
-export_thm is_position_def;;
+export_thm is_unicode_position_def;;
 
-let position_exists = prove
-  (`?p. is_position p`,
+let unicode_position_exists = prove
+  (`?p. is_unicode_position p`,
    EXISTS_TAC `p : word16` THEN
-   REWRITE_TAC [is_position_def]);;
+   REWRITE_TAC [is_unicode_position_def]);;
 
-let (position_abs_rep,position_rep_abs) =
+let (unicode_position_abs_rep,unicode_position_rep_abs) =
   let tybij =
-    new_type_definition
-      "position" ("mk_position","dest_position") position_exists in
-  CONJ_PAIR (REWRITE_RULE [is_position_def] tybij);;
+    new_type_definition "unicode_position"
+      ("mk_unicode_position","dest_unicode_position") unicode_position_exists in
+  CONJ_PAIR (REWRITE_RULE [is_unicode_position_def] tybij);;
 
-export_thm position_abs_rep;;
-export_thm position_rep_abs;;
+export_thm unicode_position_abs_rep;;
+export_thm unicode_position_rep_abs;;
 
-let position_tybij = CONJ position_abs_rep position_rep_abs;;
+let unicode_position_tybij =
+    CONJ unicode_position_abs_rep unicode_position_rep_abs;;
 
-let rdecode_position_def = new_definition
+let rdecode_unicode_position_def = new_definition
   `!r.
-     rdecode_position r =
+     rdecode_unicode_position r =
      let (w,r') = rdecode_word16 r in
-     (mk_position w, r')`;;
+     (mk_unicode_position w, r')`;;
 
-export_thm rdecode_position_def;;
+export_thm rdecode_unicode_position_def;;
 
 (* ~~~~~~~~~~~~~~~~~~ *)
 (* Unicode characters *)
@@ -90,8 +92,8 @@ export_thm rdecode_position_def;;
 let is_unicode_def = new_definition
   `!pl pos.
      is_unicode (pl,pos) =
-     let pli = dest_plane pl in
-     let posi = dest_position pos in
+     let pli = dest_unicode_plane pl in
+     let posi = dest_unicode_position pos in
      ~(pli = num_to_byte 0) \/
      word16_lt posi (num_to_word16 55296) \/
      (word16_lt (num_to_word16 57343) posi /\
@@ -101,10 +103,11 @@ export_thm is_unicode_def;;
 
 let unicode_exists = prove
   (`?pl_pos. is_unicode pl_pos`,
-   EXISTS_TAC `(mk_plane (num_to_byte 1), (pos : position))` THEN
+   EXISTS_TAC
+     `(mk_unicode_plane (num_to_byte 1), (pos : unicode_position))` THEN
    REWRITE_TAC [is_unicode_def; LET_DEF; LET_END_DEF] THEN
-   MP_TAC (SPEC `num_to_byte 1` (CONJUNCT2 plane_tybij)) THEN
-   REWRITE_TAC [is_plane_def] THEN
+   MP_TAC (SPEC `num_to_byte 1` (CONJUNCT2 unicode_plane_tybij)) THEN
+   REWRITE_TAC [is_unicode_plane_def] THEN
    CONV_TAC byte_reduce_conv THEN
    STRIP_TAC THEN
    ASM_REWRITE_TAC [] THEN
@@ -124,13 +127,13 @@ let unicode_tybij = CONJ unicode_abs_rep unicode_rep_abs;;
 let rdecode_unicode_def = new_definition
   `!r.
      rdecode_unicode r =
-     let (pl,r') = rdecode_plane r in
-     let pli = dest_plane pl in
+     let (pl,r') = rdecode_unicode_plane r in
+     let pli = dest_unicode_plane pl in
      let (pos,r'') =
-         if ~(pli = num_to_byte 0) then rdecode_position r' else
+         if ~(pli = num_to_byte 0) then rdecode_unicode_position r' else
          let (n,r''') = rdecode_uniform 63486 r' in
          let n' = if n < 55296 then n else n + 2048 in
-         (mk_position (num_to_word16 n'), r''') in
+         (mk_unicode_position (num_to_word16 n'), r''') in
      (mk_unicode (pl,pos), r'')`;;
 
 export_thm rdecode_unicode_def;;
@@ -147,66 +150,66 @@ new_type_abbrev("string",`:char list`);;
 
 logfile "char-thm";;
 
-let plane_cases = prove
-  (`!pl. ?b. is_plane b /\ pl = mk_plane b`,
+let unicode_plane_cases = prove
+  (`!pl. ?b. is_unicode_plane b /\ pl = mk_unicode_plane b`,
    GEN_TAC THEN
-   EXISTS_TAC `dest_plane pl` THEN
-   REWRITE_TAC [plane_tybij]);;
+   EXISTS_TAC `dest_unicode_plane pl` THEN
+   REWRITE_TAC [unicode_plane_tybij]);;
 
-export_thm plane_cases;;
+export_thm unicode_plane_cases;;
 
-let dest_plane_cases = prove
-  (`!pl. ?b. is_plane b /\ pl = mk_plane b /\ dest_plane pl = b`,
+let dest_unicode_plane_cases = prove
+  (`!pl. ?b. is_unicode_plane b /\ pl = mk_unicode_plane b /\ dest_unicode_plane pl = b`,
    GEN_TAC THEN
-   MP_TAC (SPEC `pl : plane` plane_cases) THEN
-   REWRITE_TAC [plane_tybij] THEN
+   MP_TAC (SPEC `pl : unicode_plane` unicode_plane_cases) THEN
+   REWRITE_TAC [unicode_plane_tybij] THEN
    STRIP_TAC THEN
    EXISTS_TAC `b : byte` THEN
    ASM_REWRITE_TAC []);;
 
-export_thm dest_plane_cases;;
+export_thm dest_unicode_plane_cases;;
 
-let dest_plane_inj = prove
-  (`!pl1 pl2. dest_plane pl1 = dest_plane pl2 <=> pl1 = pl2`,
+let dest_unicode_plane_inj = prove
+  (`!pl1 pl2. dest_unicode_plane pl1 = dest_unicode_plane pl2 <=> pl1 = pl2`,
    REPEAT GEN_TAC THEN
    EQ_TAC THENL
    [STRIP_TAC THEN
-    ONCE_REWRITE_TAC [GSYM plane_abs_rep] THEN
+    ONCE_REWRITE_TAC [GSYM unicode_plane_abs_rep] THEN
     ASM_REWRITE_TAC [];
     STRIP_TAC THEN
     ASM_REWRITE_TAC []]);;
 
-export_thm dest_plane_inj;;
+export_thm dest_unicode_plane_inj;;
 
-let position_cases = prove
-  (`!pos. ?w. pos = mk_position w`,
+let unicode_position_cases = prove
+  (`!pos. ?w. pos = mk_unicode_position w`,
    GEN_TAC THEN
-   EXISTS_TAC `dest_position pos` THEN
-   REWRITE_TAC [position_tybij]);;
+   EXISTS_TAC `dest_unicode_position pos` THEN
+   REWRITE_TAC [unicode_position_tybij]);;
 
-export_thm position_cases;;
+export_thm unicode_position_cases;;
 
-let dest_position_cases = prove
-  (`!pos. ?w. pos = mk_position w /\ dest_position pos = w`,
+let dest_unicode_position_cases = prove
+  (`!pos. ?w. pos = mk_unicode_position w /\ dest_unicode_position pos = w`,
    GEN_TAC THEN
-   MP_TAC (SPEC `pos : position` position_cases) THEN
+   MP_TAC (SPEC `pos : unicode_position` unicode_position_cases) THEN
    STRIP_TAC THEN
    EXISTS_TAC `w : word16` THEN
-   ASM_REWRITE_TAC [position_tybij]);;
+   ASM_REWRITE_TAC [unicode_position_tybij]);;
 
-export_thm dest_position_cases;;
+export_thm dest_unicode_position_cases;;
 
-let dest_position_inj = prove
-  (`!pos1 pos2. dest_position pos1 = dest_position pos2 <=> pos1 = pos2`,
+let dest_unicode_position_inj = prove
+  (`!pos1 pos2. dest_unicode_position pos1 = dest_unicode_position pos2 <=> pos1 = pos2`,
    REPEAT GEN_TAC THEN
    EQ_TAC THENL
    [STRIP_TAC THEN
-    ONCE_REWRITE_TAC [GSYM position_abs_rep] THEN
+    ONCE_REWRITE_TAC [GSYM unicode_position_abs_rep] THEN
     ASM_REWRITE_TAC [];
     STRIP_TAC THEN
     ASM_REWRITE_TAC []]);;
 
-export_thm dest_position_inj;;
+export_thm dest_unicode_position_inj;;
 
 let unicode_cases = prove
   (`!c. ?pl pos. is_unicode (pl,pos) /\ c = mk_unicode (pl,pos)`,
@@ -225,8 +228,8 @@ let dest_unicode_cases = prove
    MP_TAC (SPEC `c : unicode` unicode_cases) THEN
    REWRITE_TAC [unicode_tybij] THEN
    STRIP_TAC THEN
-   EXISTS_TAC `pl : plane` THEN
-   EXISTS_TAC `pos : position` THEN
+   EXISTS_TAC `pl : unicode_plane` THEN
+   EXISTS_TAC `pos : unicode_position` THEN
    ASM_REWRITE_TAC []);;
 
 export_thm dest_unicode_cases;;
@@ -272,7 +275,7 @@ export_thm parse_cont3_def;;
 let decode_cont1_def = new_definition
   `!b0 b1.
      decode_cont1 b0 b1 =
-     let pl = mk_plane (num_to_byte 0) in
+     let pl = mk_unicode_plane (num_to_byte 0) in
      let p1 = byte_shr (byte_and b0 (num_to_byte 28)) 2 in
      let y0 = byte_shl (byte_and b0 (num_to_byte 3)) 6 in
      let x0 = byte_and b1 (num_to_byte 63) in
@@ -280,7 +283,7 @@ let decode_cont1_def = new_definition
      if p1 = num_to_byte 0 /\ ~byte_bit p0 7 then
        NONE
      else
-       let pos = mk_position (bytes_to_word16 p0 p1) in
+       let pos = mk_unicode_position (bytes_to_word16 p0 p1) in
        let ch = mk_unicode (pl,pos) in
        SOME ch`;;
 
@@ -301,8 +304,8 @@ let decode_cont2_def = new_definition
        let p0 = byte_or y0 x0 in
        if p1 = num_to_byte 255 /\ byte_le (num_to_byte 254) p0 then NONE
        else
-         let pl = mk_plane (num_to_byte 0) in
-         let pos = mk_position (bytes_to_word16 p0 p1) in
+         let pl = mk_unicode_plane (num_to_byte 0) in
+         let pos = mk_unicode_position (bytes_to_word16 p0 p1) in
          let ch = mk_unicode (pl,pos) in
          SOME ch`;;
 
@@ -316,14 +319,14 @@ let decode_cont3_def = new_definition
      let p = byte_or w z in
      if p = num_to_byte 0 \/ byte_lt (num_to_byte 16) p then NONE
      else
-       let pl = mk_plane p in
+       let pl = mk_unicode_plane p in
        let z1 = byte_shl (byte_and b1 (num_to_byte 15)) 4 in
        let y1 = byte_shr (byte_and b2 (num_to_byte 60)) 2 in
        let p1 = byte_or z1 y1 in
        let y0 = byte_shl (byte_and b2 (num_to_byte 3)) 6 in
        let x0 = byte_and b3 (num_to_byte 63) in
        let p0 = byte_or y0 x0 in
-       let pos = mk_position (bytes_to_word16 p0 p1) in
+       let pos = mk_unicode_position (bytes_to_word16 p0 p1) in
        let ch = mk_unicode (pl,pos) in
        SOME ch`;;
 
@@ -345,8 +348,8 @@ let decoder_parse_def = new_definition
        else
          NONE
      else
-       let pl = mk_plane (num_to_byte 0) in
-       let pos = mk_position (bytes_to_word16 b0 (num_to_byte 0)) in
+       let pl = mk_unicode_plane (num_to_byte 0) in
+       let pos = mk_unicode_position (bytes_to_word16 b0 (num_to_byte 0)) in
        let ch = mk_unicode (pl,pos) in
        SOME (ch,s)`;;
 
@@ -414,8 +417,8 @@ let encoder_def = new_definition
   `!ch.
      encoder ch =
      let (pl,pos) = dest_unicode ch in
-     let p = dest_plane pl in
-     let (p0,p1) = word16_to_bytes (dest_position pos) in
+     let p = dest_unicode_plane pl in
+     let (p0,p1) = word16_to_bytes (dest_unicode_position pos) in
      if p = num_to_byte 0 then
        if p1 = num_to_byte 0 /\ ~byte_bit p0 7 then
          CONS p0 []
@@ -510,11 +513,11 @@ let decoder_encoder_inverse = prove
    POP_ASSUM (fun th -> REWRITE_TAC [th]) THEN
    POP_ASSUM (fun th -> REWRITE_TAC [th]) THEN
    POP_ASSUM MP_TAC THEN
-   MP_TAC (SPEC `pl : plane` dest_plane_cases) THEN
+   MP_TAC (SPEC `pl : unicode_plane` dest_unicode_plane_cases) THEN
    DISCH_THEN (X_CHOOSE_THEN `p : byte` STRIP_ASSUME_TAC) THEN
    POP_ASSUM (fun th -> REWRITE_TAC [th]) THEN
    POP_ASSUM (fun th -> REWRITE_TAC [th]) THEN
-   MP_TAC (SPEC `pos : position` dest_position_cases) THEN
+   MP_TAC (SPEC `pos : unicode_position` dest_unicode_position_cases) THEN
    STRIP_TAC THEN
    POP_ASSUM (fun th -> REWRITE_TAC [th]) THEN
    POP_ASSUM (fun th -> REWRITE_TAC [th]) THEN
@@ -618,9 +621,9 @@ let decoder_encoder_inverse = prove
       DISCH_THEN MATCH_MP_TAC THEN
       CONJ_TAC THENL
       [PAT_ASSUM `is_unicode X` THEN
-       ASM_REWRITE_TAC [is_unicode_def; position_tybij] THEN
-       PAT_ASSUM `is_plane X` THEN
-       REWRITE_TAC [plane_tybij] THEN
+       ASM_REWRITE_TAC [is_unicode_def; unicode_position_tybij] THEN
+       PAT_ASSUM `is_unicode_plane X` THEN
+       REWRITE_TAC [unicode_plane_tybij] THEN
        DISCH_THEN (fun th -> REWRITE_TAC [th]) THEN
        bit_blast_tac THEN
        REWRITE_TAC [LET_DEF; LET_END_DEF] THEN
@@ -635,9 +638,9 @@ let decoder_encoder_inverse = prove
        ALL_TAC] THEN
       DISCH_THEN MATCH_MP_TAC THEN
       PAT_ASSUM `is_unicode X` THEN
-      ASM_REWRITE_TAC [is_unicode_def; position_tybij] THEN
-      PAT_ASSUM `is_plane X` THEN
-      ASM_REWRITE_TAC [plane_tybij] THEN
+      ASM_REWRITE_TAC [is_unicode_def; unicode_position_tybij] THEN
+      PAT_ASSUM `is_unicode_plane X` THEN
+      ASM_REWRITE_TAC [unicode_plane_tybij] THEN
       DISCH_THEN (fun th -> REWRITE_TAC [th]) THEN
       bit_blast_tac THEN
       REWRITE_TAC [LET_DEF; LET_END_DEF] THEN
@@ -690,8 +693,8 @@ let decoder_encoder_inverse = prove
      ALL_TAC] THEN
     DISCH_THEN MATCH_MP_TAC THEN
     CONJ_TAC THENL
-    [PAT_ASSUM `is_plane X` THEN
-     ASM_REWRITE_TAC [is_plane_def] THEN
+    [PAT_ASSUM `is_unicode_plane X` THEN
+     ASM_REWRITE_TAC [is_unicode_plane_def] THEN
      bit_blast_tac THEN
      ASM_TAUT_TAC;
      ALL_TAC] THEN
@@ -702,8 +705,8 @@ let decoder_encoder_inverse = prove
     AP_THM_TAC THEN
     AP_TERM_TAC THEN
     AP_TERM_TAC THEN
-    PAT_ASSUM `is_plane X` THEN
-    ASM_REWRITE_TAC [is_plane_def] THEN
+    PAT_ASSUM `is_unicode_plane X` THEN
+    ASM_REWRITE_TAC [is_unicode_plane_def] THEN
     bit_blast_tac THEN
     ASM_TAUT_TAC]);;
 
@@ -876,19 +879,19 @@ let decoder_encoder_strong_inverse = prove
        REWRITE_TAC [GSYM unicode_rep_abs] THEN
        KNOW_TAC
          `!x y z.
-            is_plane x /\
-            (is_plane x ==>
-             is_unicode (mk_plane x, mk_position y) /\ z) ==>
-            is_unicode (mk_plane x, mk_position y) /\ z` THENL
+            is_unicode_plane x /\
+            (is_unicode_plane x ==>
+             is_unicode (mk_unicode_plane x, mk_unicode_position y) /\ z) ==>
+            is_unicode (mk_unicode_plane x, mk_unicode_position y) /\ z` THENL
        [SIMP_TAC [];
         ALL_TAC] THEN
        DISCH_THEN MATCH_MP_TAC THEN
        CONJ_TAC THENL
-       [REWRITE_TAC [is_plane_def] THEN
+       [REWRITE_TAC [is_unicode_plane_def] THEN
         bit_blast_tac;
         ALL_TAC] THEN
-       REWRITE_TAC [is_unicode_def; position_tybij] THEN
-       DISCH_THEN (fun th -> REWRITE_TAC [REWRITE_RULE [plane_tybij] th]) THEN
+       REWRITE_TAC [is_unicode_def; unicode_position_tybij] THEN
+       DISCH_THEN (fun th -> REWRITE_TAC [REWRITE_RULE [unicode_plane_tybij] th]) THEN
        SUBGOAL_THEN
          `(list_to_byte
              [b14; b15; b00; b01; ~b01 /\ ~b00 /\ ~b15 /\ ~b14; F; F; F] =
@@ -1006,19 +1009,19 @@ let decoder_encoder_strong_inverse = prove
        REWRITE_TAC [GSYM unicode_rep_abs] THEN
        KNOW_TAC
          `!x y z.
-            is_plane x /\
-            (is_plane x ==>
-             is_unicode (mk_plane x, mk_position y) /\ z) ==>
-            is_unicode (mk_plane x, mk_position y) /\ z` THENL
+            is_unicode_plane x /\
+            (is_unicode_plane x ==>
+             is_unicode (mk_unicode_plane x, mk_unicode_position y) /\ z) ==>
+            is_unicode (mk_unicode_plane x, mk_unicode_position y) /\ z` THENL
        [SIMP_TAC [];
         ALL_TAC] THEN
        DISCH_THEN MATCH_MP_TAC THEN
        CONJ_TAC THENL
-       [REWRITE_TAC [is_plane_def] THEN
+       [REWRITE_TAC [is_unicode_plane_def] THEN
         bit_blast_tac;
         ALL_TAC] THEN
-       REWRITE_TAC [is_unicode_def; position_tybij] THEN
-       DISCH_THEN (fun th -> REWRITE_TAC [REWRITE_RULE [plane_tybij] th]) THEN
+       REWRITE_TAC [is_unicode_def; unicode_position_tybij] THEN
+       DISCH_THEN (fun th -> REWRITE_TAC [REWRITE_RULE [unicode_plane_tybij] th]) THEN
        CONJ_TAC THENL
        [REWRITE_TAC [LET_DEF; LET_END_DEF] THEN
         DISJ2_TAC THEN
@@ -1108,19 +1111,19 @@ let decoder_encoder_strong_inverse = prove
       REWRITE_TAC [GSYM unicode_rep_abs] THEN
       KNOW_TAC
         `!x y z.
-           is_plane x /\
-           (is_plane x ==>
-            is_unicode (mk_plane x, mk_position y) /\ z) ==>
-           is_unicode (mk_plane x, mk_position y) /\ z` THENL
+           is_unicode_plane x /\
+           (is_unicode_plane x ==>
+            is_unicode (mk_unicode_plane x, mk_unicode_position y) /\ z) ==>
+           is_unicode (mk_unicode_plane x, mk_unicode_position y) /\ z` THENL
       [SIMP_TAC [];
        ALL_TAC] THEN
       DISCH_THEN MATCH_MP_TAC THEN
       CONJ_TAC THENL
-      [REWRITE_TAC [is_plane_def] THEN
+      [REWRITE_TAC [is_unicode_plane_def] THEN
        bit_blast_tac;
        ALL_TAC] THEN
-      REWRITE_TAC [is_unicode_def; position_tybij] THEN
-      DISCH_THEN (fun th -> REWRITE_TAC [REWRITE_RULE [plane_tybij] th]) THEN
+      REWRITE_TAC [is_unicode_def; unicode_position_tybij] THEN
+      DISCH_THEN (fun th -> REWRITE_TAC [REWRITE_RULE [unicode_plane_tybij] th]) THEN
       CONJ_TAC THENL
       [REWRITE_TAC [LET_DEF; LET_END_DEF] THEN
        DISJ2_TAC THEN
@@ -1160,19 +1163,19 @@ let decoder_encoder_strong_inverse = prove
     REWRITE_TAC [GSYM unicode_rep_abs] THEN
     KNOW_TAC
       `!x y z.
-         is_plane x /\
-         (is_plane x ==>
-          is_unicode (mk_plane x, mk_position y) /\ z) ==>
-         is_unicode (mk_plane x, mk_position y) /\ z` THENL
+         is_unicode_plane x /\
+         (is_unicode_plane x ==>
+          is_unicode (mk_unicode_plane x, mk_unicode_position y) /\ z) ==>
+         is_unicode (mk_unicode_plane x, mk_unicode_position y) /\ z` THENL
     [SIMP_TAC [];
      ALL_TAC] THEN
     DISCH_THEN MATCH_MP_TAC THEN
     CONJ_TAC THENL
-    [REWRITE_TAC [is_plane_def] THEN
+    [REWRITE_TAC [is_unicode_plane_def] THEN
      bit_blast_tac;
      ALL_TAC] THEN
-    REWRITE_TAC [is_unicode_def; position_tybij] THEN
-    DISCH_THEN (fun th -> REWRITE_TAC [REWRITE_RULE [plane_tybij] th]) THEN
+    REWRITE_TAC [is_unicode_def; unicode_position_tybij] THEN
+    DISCH_THEN (fun th -> REWRITE_TAC [REWRITE_RULE [unicode_plane_tybij] th]) THEN
     CONJ_TAC THENL
     [REWRITE_TAC [LET_DEF; LET_END_DEF] THEN
      DISJ2_TAC THEN
